PREFIX : <https://linked.data.gov.au/def/abis/vocab-themes/>
PREFIX cs: <https://linked.data.gov.au/def/abis/vocab-themes>
PREFIX rdfs: <http://www.w3.org/2000/01/rdf-schema#>
PREFIX schema: <https://schema.org/>
PREFIX skos: <http://www.w3.org/2004/02/skos/core#>
PREFIX xsd: <http://www.w3.org/2001/XMLSchema#>


cs:
    a skos:ConceptScheme ;
    skos:hasTopConcept
        :datatypes ,
        :data-roles ,
        :feature-types ,
        :observation-types ,
        :observable-properties ,
        :procedures ,
        :sampling-types ;
    skos:prefLabel "ABIS Vocabulary Themes"@en;
    skos:definition "This vocabulary contains themes that vocabularies by data created according to the the Australian Biodiversity Information Standard (ABIS) are categorised with." ;
    schema:creator <https://linked.data.gov.au/org/dcceew> ;
    schema:publisher <https://linked.data.gov.au/org/dcceew> ;
    schema:dateCreated "2024-06-21"^^xsd:date ;
    schema:dateModified "2025-04-16"^^xsd:date ;
    schema:license <http://purl.org/NET/rdflicense/cc-by4.0> ;
    skos:historyNote "Created by the BDR team in 2024 to assist with management of the BDR content" ;
.

<https://linked.data.gov.au/org/dcceew>
    a schema:Organization ;
    schema:name "Department of Climate Change, Energy, the Environment and Water, DCCEEW" ;
    schema:url "https://www.dcceew.gov.au"^^xsd:anyURI ;
.

:datatypes
    a skos:Concept ;
    skos:prefLabel "Data Types";
    skos:definition "Vocabularies with the dcat:theme abis/data-themes:datatypes can be used for Literal Datatypes in ABIS Datasets."@en;
    rdfs:isDefinedBy cs: ;
    skos:inScheme cs: ;
    skos:topConceptOf cs: ;
.

:data-roles 
    a skos:Concept ;
    skos:prefLabel "Data Roles";
    skos:definition "Vocabularies with the dcat:theme abis/data-themes:data-roles can be used for prov role attributions on ABIS Datasets."@en;
    rdfs:isDefinedBy cs: ;
    skos:inScheme cs: ;
    skos:topConceptOf cs: ;
.

:feature-types 
    a skos:Concept ;
    skos:prefLabel "Feature Types";
    skos:definition "Vocabularies with the dcat:theme abis/vocab-themes:feature-type can be used where concepts go in the tern:featureType slot"@en;
    rdfs:isDefinedBy cs: ;
    skos:inScheme cs: ;
    skos:topConceptOf cs: ;
.

:observable-properties 
    a skos:Concept ;
    skos:prefLabel "Observable Properties";
    skos:definition "Vocabularies with the dcat:theme abis/vocab-themes:observable-properties can be used where concepts go in observableProperty on a sosa:FeatureOfInterest or observedProperty on sosa:Observation."@en;
    rdfs:isDefinedBy cs: ;
    skos:inScheme cs: ;
    skos:topConceptOf cs: ;
.

:observation-types
    a skos:Concept ;
    skos:prefLabel "Observation Types";
    skos:definition "Vocabularies with the dcat:theme abis/vocab-themes:observation-type can be used where concepts go in the tern:observationType or sdo:additionalType slot on a tern:Observation or sosa:Observation."@en;
    rdfs:isDefinedBy cs: ;
    skos:inScheme cs: ;
    skos:topConceptOf cs: ;
.

:procedures
    a skos:Concept ;
    skos:prefLabel "Procedures";
    skos:definition "Vocabularies with the dcat:theme abis/vocab-themes:observation-type can be used where concepts go in the tern:observationType or sdo:additionalType slot on a tern:Observation or sosa:Observation."@en;
    rdfs:isDefinedBy cs: ;
    skos:inScheme cs: ;
    skos:topConceptOf cs: ;
.

:sampling-types
    a skos:Concept ;
    skos:prefLabel "Sampling Types";
    skos:definition "Vocabularies with the dcat:theme abis/vocab-themes:sample-type can be used where concepts go in the tern:samplingType or sdo:additionalType slot on a tern:Sampling or sosa:Sampling."@en;
    rdfs:isDefinedBy cs: ;
    skos:inScheme cs: ;
    skos:topConceptOf cs: ;
.
