@prefix skos: <http://www.w3.org/2004/02/skos/core#> .
@prefix cs: <https://linked.data.gov.au/def/abis/vocab-themes> .
@prefix : <https://linked.data.gov.au/def/abis/vocab-themes/> .


cs: a skos:ConceptScheme ;
    skos:hasTopConcept :feature-types ;
    skos:hasTopConcept :sampling-types ;
    skos:hasTopConcept :data-roles ;
    skos:hasTopConcept :datatypes ;
    skos:hasTopConcept :procedures ;
    skos:hasTopConcept :observation-types ;
    skos:hasTopConcept :observable-properties ;
    skos:prefLabel "ABIS Themed-Vocabulary Themes"@en;
    .

:data-roles a skos:Concept ;
    skos:prefLabel "ABIS Vocab Theme: Data Roles";
    skos:definition "Vocabularies with the dcat:theme abis/data-themes:data-roles can be used for prov role attributions on ABIS Datasets."@en;
    skos:topConceptOf cs: ;
    .

:datatypes a skos:Concept ;
    skos:prefLabel "ABIS Vocab Theme: Data Types";
    skos:definition "Vocabularies with the dcat:theme abis/data-themes:datatypes can be used for Literal Datatypes in ABIS Datasets."@en;
    skos:topConceptOf cs: ;
    .

:feature-types a skos:Concept ;
    skos:prefLabel "ABIS Vocab Theme: Feature Types";
    skos:definition "Vocabularies with the dcat:theme abis/vocab-themes:feature-type can be used where concepts go in the tern:featureType slot"@en;
    skos:topConceptOf cs: ;
    .

:sampling-types a skos:Concept ;
    skos:prefLabel "ABIS Vocab Theme: Sampling Types";
    skos:definition "Vocabularies with the dcat:theme abis/vocab-themes:sample-type can be used where concepts go in the tern:samplingType or sdo:additionalType slot on a tern:Sampling or sosa:Sampling."@en;
    skos:topConceptOf cs: ;
    .

:observation-types a skos:Concept ;
    skos:prefLabel "ABIS Vocab Theme: Observation Types";
    skos:definition "Vocabularies with the dcat:theme abis/vocab-themes:observation-type can be used where concepts go in the tern:observationType or sdo:additionalType slot on a tern:Observation or sosa:Observation."@en;
    skos:topConceptOf cs: ;
    .

:procedures a skos:Concept ;
    skos:prefLabel "ABIS Vocab Theme: Procedures";
    skos:definition "Vocabularies with the dcat:theme abis/vocab-themes:observation-type can be used where concepts go in the tern:observationType or sdo:additionalType slot on a tern:Observation or sosa:Observation."@en;
    skos:topConceptOf cs: ;
    .

:observable-properties a skos:Concept ;
    skos:prefLabel "ABIS Vocab Theme: Observable Properties";
    skos:definition "Vocabularies with the dcat:theme abis/vocab-themes:observable-properties can be used where concepts go in observableProperty on a sosa:FeatureOfInterest or observedProperty on sosa:Observation."@en;
    skos:topConceptOf cs: ;
    .
